feature: memories store labeled values rather than ownership

src/x86/Architecture/Architecture_func.v
@@ -1,96 +1,113 @@
 Require Import SpecCert.x86.Architecture.ProcessorUnit.
 Require Import SpecCert.x86.Architecture.MemoryController.
 Require Import SpecCert.x86.Architecture.Architecture_rec.
+Require Import SpecCert.x86.Value.
 Require Import SpecCert.Memory.
 Require Import SpecCert.Address.
 Require Import SpecCert.Cache.
 
-Definition update_proc
-           {S  :Set}
-           (a  :Architecture S)
-           (p' :ProcessorUnit) :=
+Program Definition update_proc
+        {Label: Type}
+        (a:     Architecture Label)
+        (p':    ProcessorUnit) :=
   {| proc              := p'
    ; memory_controller := (memory_controller a)
    ; memory            := (memory a)
-   ; cache             := (cache a) |}.
+   ; cache             := (cache a)
+   |}.
+Next Obligation.
+  apply (x86_cache_is_well_formed a).
+Qed.
 
-Definition update_memory_controller
-           {S  :Set}
-           (a  :Architecture S)
-           (m' :MemoryController) :=
+Program Definition update_memory_controller
+        {Label: Type}
+        (a:     Architecture Label)
+        (m':    MemoryController) :=
   {| proc              := (proc a)
    ; memory_controller := m'
    ; memory            := (memory a)
-   ; cache             := (cache a) |}.
+   ; cache             := (cache a)
+   |}.
+Next Obligation.
+  apply (x86_cache_is_well_formed a).
+Qed.
 
-Definition update_memory_content
-           {S  :Set}
-           (a  :Architecture S)
-           (ha :HardwareAddress)
-           (c  :S) :=
+Program Definition update_memory_content
+        {Label: Type}
+        (a:     Architecture Label)
+        (ha:    HardwareAddress)
+        (c:     (Value*Label)) :=
   {| proc              := (proc a)
    ; memory_controller := (memory_controller a)
    ; memory            := (update_in_memory (memory a) ha c)
-   ; cache             := (cache a) |}.
+   ; cache             := (cache a)
+   |}.
+Next Obligation.
+  apply (x86_cache_is_well_formed a).
+Qed.
 
 Definition find_memory_content
-           {S  :Set}
-           (a  :Architecture S)
-           (ha :HardwareAddress)
-           :S :=
+           {Label: Type}
+           (a:     Architecture Label)
+           (ha:    HardwareAddress)
+  : (Value * Label) :=
   find_in_memory (memory a) ha.
 
 Definition phys_to_hard
-           {S  :Set}
-           (a  :Architecture S)
-           (pa :PhysicalAddress)
-           :HardwareAddress :=
+           {Label: Type}
+           (a:     Architecture Label)
+           (pa:    PhysicalAddress)
+  : HardwareAddress :=
   let smiact := in_smm (proc a) in
   translate_physical_address (memory_controller a) smiact pa.
 
 Definition find_cache_content
-           {S  :Set}
-           (a  :Architecture S)
-           (pa :PhysicalAddress)
-           :option S :=
+           {Label: Type}
+           (a:     Architecture Label)
+           (pa:    PhysicalAddress)
+  : option (Value * Label) :=
   find_in_cache (cache a) pa.
 
 Definition find_cache_location_content
-           {S  :Set}
-           (a  :Architecture S)
-           (pa :PhysicalAddress)
-           :S :=
+           {Label: Type}
+           (a:  Architecture Label)
+           (pa: PhysicalAddress)
+  : (Value * Label) :=
   find_in_cache_location (cache a) pa.
 
-Definition update_cache_content
-           {S  :Set}
-           (a  :Architecture S)
-           (pa :PhysicalAddress)
-           (c  :S) :=
+Program Definition update_cache_content
+        {Label: Type}
+        (a:     Architecture Label)
+        (pa:    PhysicalAddress)
+        (c:     (Value*Label)) :=
   {| proc              := (proc a)
    ; memory_controller := (memory_controller a)
    ; memory            := (memory a)
-   ; cache             := global_update_in_cache (cache a) pa c |}.
+   ; cache             := global_update_in_cache (cache a) pa c
+   |}.
+Next Obligation.
+  remember (global_update_in_cache (cache a) pa (v, l)) as cache'.
+  apply (cache_stays_well_formed (cache a) cache' pa  (v, l) (x86_cache_is_well_formed a) Heqcache').
+Qed.
 
 Definition load_in_cache_from_memory
-           {S  :Set}
-           (a  :Architecture S)
-           (pa :PhysicalAddress)
-           :Architecture S :=
-  let cont := find_in_cache_location (cache a) pa in
-  let cont' := find_memory_content a (phys_to_hard a pa) in
+           {Label: Type}
+           (a:     Architecture Label)
+           (pa:    PhysicalAddress) :=
   let a' := if cache_location_is_dirty_dec (cache a) pa
             then let pa' := cache_location_address (cache a) pa in
                  let ha := phys_to_hard a pa' in
+                 let cont := find_in_cache_location (cache a) pa in
                  update_memory_content a ha cont
             else a in
+  let cont' := find_memory_content a' (phys_to_hard a' pa) in
   update_cache_content a' pa cont'.
 
 Definition find_address_content
-           {S  :Set}
-           (a  :Architecture S)
-           (pa :PhysicalAddress)
-           :option S :=
+           {Label: Type}
+           (a:     Architecture Label)
+           (pa:    PhysicalAddress)
+  : option (Value*Label) :=
   match (resolve_cache_strategy (proc a) pa) with
   | Uncachable => Some (find_memory_content a (phys_to_hard a pa))
   | SmrrHit    => None
@@ -98,10 +115,3 @@ Definition find_address_content
                  then Some (find_in_cache_location (cache a) pa)
                  else Some (find_memory_content a (phys_to_hard a pa))
   end.
-
-(*
-Definition context (p :ProcessorUnit) :=
-  if is_in_smm_dec p
-  then smm
-  else ring0.
-*)
