src/x86/Transition/Event/Write.v
@@ -1,42 +1,45 @@
 Require Import SpecCert.x86.Architecture.
 Require Import SpecCert.Address.
 Require Import SpecCert.Cache.
+Require Import SpecCert.x86.Value.
 
 Definition write_uncachable
-           {S        :Set}
-           (a        :Architecture S)
-           (context  :Architecture S -> S)
-           (pa       :PhysicalAddress) :=
-  let current_context := (context a) in
+           {Label:    Type}
+           (a:        Architecture Label)
+           (labelize: Architecture Label -> Label)
+           (pa:       PhysicalAddress)
+           (val:      Value) :=
+  let lab := (labelize a) in
   let ha := phys_to_hard a pa in
-  update_memory_content a ha current_context.
+  update_memory_content a ha (val,lab).
 
 Definition write_writeback
-           {S        :Set}
-           (a        :Architecture S)
-           (context  :Architecture S -> S)
-           (pa       :PhysicalAddress) :=
-  let current_context := (context a) in
+           {Label:    Type}
+           (a:        Architecture Label)
+           (labelize: Architecture Label -> Label)
+           (pa:       PhysicalAddress)
+           (val:      Value) :=
+  let lab := (labelize a) in
   let a' := if cache_hit_dec (cache a) pa
             then a
             else load_in_cache_from_memory a pa in
-  update_cache_content a' pa current_context.
+  update_cache_content a' pa (val,lab).
 
 (* Intel, Chapter 11: Memory Cache Control
   "If the logical processor is not in SMM, write accesses are ignored (...)" *)
 Definition write_smrrhit
-           {S  :Set}
-           (a  :Architecture S)
-           (pa :PhysicalAddress) :=
+           {Label:    Type}
+           (a:        Architecture Label) :=
   a.
 
 Definition write_post
-           {S       :Set}
-           (context :Architecture S -> S)
-           (pa      :PhysicalAddress) :=
-  fun (a a':Architecture S) =>
-    match resolve_cache_strategy (proc a) pa with
-    | Uncachable => a' = write_uncachable a context pa
-    | WriteBack  => a' = write_writeback a context pa
-    | SmrrHit    => a' = write_smrrhit a pa
-    end.
+           {Label:    Type}
+           (labelize: Architecture Label -> Label)
+           (pa:       PhysicalAddress)
+           (val:      Value)
+           (a a':Architecture Label) :=
+  match resolve_cache_strategy (proc a) pa with
+  | Uncachable => a' = write_uncachable a labelize pa val
+  | WriteBack  => a' = write_writeback a labelize pa val
+  | SmrrHit    => a' = write_smrrhit a
+  end.
