src/x86/Architecture/Architecture_rec.v
@@ -3,26 +3,20 @@ Require Import SpecCert.x86.Architecture.MemoryController.
 Require Import SpecCert.Address.
 Require Import SpecCert.Memory.
 Require Import SpecCert.Cache.
+Require Import SpecCert.x86.Value.
 
-Record Architecture (S:Set) :=
-  { proc: ProcessorUnit
+Record Architecture (Label: Type) :=
+  { proc:              ProcessorUnit
   ; memory_controller: MemoryController
-  ; memory: Memory S
-  ; cache: Cache S }.
+  ; memory:            Memory (Value * Label)
+  ; cache:             Cache (Value * Label)
+  ; x86_cache_is_well_formed:
+                       cache_is_well_formed (cache)
+  }.
 
-Arguments cache : default implicits.
-Arguments memory : default implicits.
-Arguments memory_controller : default implicits.
-Arguments proc : default implicits.
-
-(* This axiom is justified by the following lemma:
-   `cache_stays_well_formed` (src/Cache/Cache_proofs.v).
-   Indeed, we only use global_update_in_cache in order
-   to modify the cache.
-
-   Note that it could be added as invariant. In order to
-   simplify the proof, we don't. But it could be a TODO.
- *)
-Axiom hardware_ensures_cache_is_well_formed:
-  forall S:Set, forall a:Architecture S,
-    cache_is_well_formed (cache a).
+Arguments cache:             default implicits.
+Arguments memory:            default implicits.
+Arguments memory_controller: default implicits.
+Arguments proc:              default implicits.
+Arguments x86_cache_is_well_formed:
+                             default implicits.
