src/x86/Transition/Event/NextInstruction.v
@@ -2,7 +2,7 @@ Require Import SpecCert.x86.Architecture.
 Require Import SpecCert.Address.
 
 Definition nextinstr_post
-           {S  :Set}
-           (pa :PhysicalAddress) :=
-  fun (a a':Architecture S) =>
-    a' = update_proc a (next_instruction (proc a) pa).
+           {Label: Type}
+           (pa: PhysicalAddress)
+           (a a':Architecture Label) :=
+  a' = update_proc a (next_instruction (proc a) pa).
